Minor cleanups to Spectra (#175)
* CLEAN prefer [#[program]] to [Program]

* Formalize the concept of mask validity

* Update rocq-skylabs-iris/theories/base_logic/lib/spectra.v

Docs point to [valid]

Co-authored-by: Paolo G. Giarrusso <paolo@skylabs-ai.com>

* Apply suggestion from @pgiarrusso-sl

* Apply suggestion from @pgiarrusso-sl

---------

Co-authored-by: Paolo G. Giarrusso <paolo@skylabs-ai.com>

rocq-skylabs-iris/theories/base_logic/lib/spectra.v
@@ -108,7 +108,8 @@ Module masks.
   (**
   A consistent choice of masks.
   When proving requesters, clients can use their own invariants with mask [E : coPset],
-  such that [E ⊆ O \ ↑refinement_rootNS] and [I ⊆ O \ ↑refinement_rootNS \ E].
+  When proving requesters for [m : masks.t], clients can use their own invariants with mask [E : coPset],
+  such that [valid m E].
   *)
   Record t : Set := {
     O : coPset; (** [O]uter mask *)
@@ -117,7 +118,7 @@ Module masks.
     RinO : ↑refinement_rootNS ⊆ O;
   }.
 
-  Program Definition default := {|
+  #[program] Definition default := {|
     O := ⊤ ;
     I := ∅ ;
   |}.
@@ -129,6 +130,19 @@ Module masks.
   Module hints.
     #[export] Hint Resolve order RinO : ndisj.
   End hints.
+
+  Definition valid (m : t) (E : coPset) : Prop :=
+    E ⊆ m.(O) ∖ ↑refinement_rootNS /\ m.(I) ⊆ m.(O) ∖ ↑refinement_rootNS ∖ E.
+
+  (** Proof that any <E> not including the refinement namespace is valid
+      relative to the default masks.
+
+      It is easy to satisfy the side condition by prefixing E with something,
+      e.g. <"impl"> for "implementation namespaces".
+   *)
+  Lemma default_valid : forall E, E ∩ ↑refinement_rootNS = ∅ -> valid default E.
+  Proof. rewrite /valid. intros. set_solver. Qed.
+
 End masks.
 Import masks.hints.
 Implicit Type (m : masks.t).
